Common_Proof.thy
@@ -41,99 +41,95 @@ next
       case (Cons a as)
       then show ?case
         apply auto
-        (* TODO: *)
-        by (smt (verit, del_insts) Nat.add_diff_assoc add.commute add_Suc diff_is_0_eq' drop_Cons' le_add1 le_add_diff_inverse2 length_Cons length_append length_drop length_rev nat_less_le not_le size_listLength)
-    qed
+       (* TODO: *)
+        by (metis length_Cons length_take size_listLength)
+     qed
   qed
 qed
+
+value "tick ( Copy (Current [] 0 (Stack [] [a\<^sub>1]) 1) [a\<^sub>2, a\<^sub>1] [] 0)"
   
 lemma invariant_push: "invariant common \<Longrightarrow> invariant (push x common)"
   apply(induction x common rule: push.induct)
   by(auto split: stack.splits current.splits)
 
+lemma helper_x: " \<not> Stack.isEmpty stack \<Longrightarrow> Suc (Stack.size (Stack.pop stack) + x) = Stack.size stack + x"
+  apply(induction stack rule: Stack.pop.induct)
+  by auto
+
+lemma helper_x2: "\<lbrakk>
+  \<not> length new < Stack.size (Stack.pop old);
+  \<not> length new < Stack.size old;
+  \<not> Stack.isEmpty old;
+  Stack.toList old = take (Stack.size old) (drop (length aux + length new - remained) (rev aux)) @ take (Stack.size old + length new - remained) new;
+  x = first old;
+  common' = Copy (Current [] 0 (Stack.pop old) (remained - Suc 0)) aux new (length new); 
+  length new < remained; 
+  moved = length new;
+  remained \<le> length aux + length new; added = 0;
+  \<not> remained - Suc 0 \<le> length new
+\<rbrakk> \<Longrightarrow> Stack.toList (Stack.pop old) =
+         take (Stack.size (Stack.pop old)) (drop (Suc (length aux + length new) - remained) (rev aux)) @
+         take (Stack.size old + length new - remained) new"
+  apply(induction old rule: Stack.pop.induct)
+    apply auto
+  apply (smt (z3) Nat.diff_diff_right Suc_diff_le diff_diff_cancel diff_is_0_eq drop_Suc drop_all_iff leD le_diff_conv length_rev less_or_eq_imp_le list.sel(3) old.nat.distinct(2) take_eq_Nil take_tl tl_append2 tl_drop)
+  (* TODO: *)
+  sorry
+
+(* TODO: *)
 lemma invariant_pop: "\<lbrakk>
   \<not> isEmpty common; 
   invariant common;
-   pop common = (x, common')
+  pop common = (x, common')
 \<rbrakk> \<Longrightarrow> invariant common'"
 proof(induction common arbitrary: x rule: pop.induct)
   case (1 current stack stackSize)
-  then show ?case 
-  proof(induction current)
-    case (Current extra added old remained)
+  then show ?case
+  proof(induction current rule: get.induct)
+    case (1 added old remained)
     then show ?case
-    proof(induction "Current extra added old remained" rule: get.induct)
-      case 1
-      then show ?case 
-      proof(induction stack arbitrary: x rule: Stack.pop.induct)
-        case (1 x left right)
-        then show ?case by auto
-      next
-        case (2 x right)
-        then show ?case
-        proof(induction old arbitrary: x rule: Stack.pop.induct)
-          case (1 x' left' right')
-          then show ?case 
-            apply auto
-            (* TODO: *)
-            by (smt (z3) Cons_nth_drop_Suc add.commute add_diff_cancel_right' diff_commute diff_less_Suc drop_Suc_Cons drop_append length_Cons length_append list.inject)
-        next
-          case (2 x' right')
-          then show ?case 
-            apply auto 
-            (* TODO: *)
-            by (metis Cons_nth_drop_Suc diff_less_Suc drop_Suc_Cons length_Cons list.sel(3))
-        next
-          case 3
-          then show ?case by auto
-        qed
-      next
-        case 3
-        then show ?case by auto
-      qed
-    next
-      case (2 x xs)
-      then show ?case
-        by(auto split: stack.splits)
-    qed
+      apply(auto split: stack.splits current.splits prod.splits)
+      apply (metis Stack.pop.simps(2) Stack.toList.simps Stack_Proof.pop append.left_neutral first_pop length_Cons size_listLength stack.inject take_tl)
+      using Stack.isEmpty.simps(1) Stack.pop.elims apply blast
+      using size_pop by fastforce
+  next
+    case (2 x xs added old remained)
+    then show ?case by(auto split: stack.splits current.splits prod.splits)
   qed
 next
   case (2 current aux new moved)
-  then show ?case 
-  (* TODO: *)
+  then show ?case
   proof(induction current rule: get.induct)
     case (1 added old remained)
-    then show ?case 
-    proof(induction "Stack.size old < length new")
+    then show ?case
+    proof(induction "length new < Stack.size old")
       case True
       then show ?case 
-        apply auto
-        apply (smt (z3) Cons_nth_drop_Suc Suc_diff_le Suc_pred diff_Suc_Suc diff_diff_cancel diff_is_0_eq' drop0 first_pop length_greater_0_conv less_imp_le list.inject not_empty_2 not_le size_listLength size_pop)
-        apply (smt (verit) Cons_nth_drop_Suc Suc_diff_le Suc_n_not_le_n add_diff_cancel_right' append_self_conv2 diff_Suc_Suc diff_is_0_eq diff_le_mono2 drop_all first_pop le_eq_less_or_eq length_rev linear list.inject minus_nat.diff_0 not_empty_2 size_pop)
-        by (meson diff_le_self le_trans)
+        apply(auto simp: size_pop)
+        apply (smt (z3) One_nat_def Suc_diff_Suc append_eq_conv_conj append_self_conv2 append_take_drop_id diff_Suc_eq_diff_pred diff_diff_cancel diff_is_0_eq' drop_Suc_Cons drop_rev first_pop le_diff_conv length_drop length_rev less_imp_le less_imp_le_nat ordered_cancel_comm_monoid_diff_class.diff_diff_right size_listLength take0 take_all)
+        apply (smt (z3) Cons_nth_drop_Suc Nat.diff_diff_right Stack_Proof.pop Suc_diff_Suc Suc_diff_le diff_less diff_zero drop_all_iff length_greater_0_conv length_rev less_add_same_cancel2 less_le_trans less_or_eq_imp_le list.sel(3) list.size(3) not_le take_eq_Nil take_tl tl_append2 zero_less_diff)
+        by (meson diff_le_self order_trans)
     next
       case False
       then show ?case
-      proof(induction "Stack.size (Stack.pop old) < length new")
-        case True
-        then show ?case 
-          apply auto
-          apply (smt (z3) append_Nil diff_add_inverse diff_diff_cancel drop0 drop_Suc_Cons drop_all first_pop le_less_Suc_eq le_refl length_Cons length_rev nat_less_le nat_neq_iff size_listLength size_pop zero_less_diff) 
-          apply (metis Suc_diff_le append_Nil diff_add_inverse2 diff_self_eq_0 drop0 drop_Suc_Cons drop_all_iff first_pop le_refl length_Cons length_rev nat_neq_iff not_less_eq size_listLength)
-          using diff_le_self le_trans by blast
-      next
-        case False
-        then show ?case 
-          apply auto
-          apply (smt (verit, ccfv_threshold) Stack_Proof.pop Suc_le_lessD Suc_pred add_diff_inverse_nat append_eq_append_conv append_take_drop_id diff_add_inverse2 drop_all_iff length_append length_drop length_greater_0_conv size_listLength size_pop tl_append2)
-          apply (smt (z3) Cons_nth_drop_Suc Suc_le_lessD diff_add_inverse2 diff_is_0_eq diff_zero drop_all_iff first_pop le_eq_less_or_eq length_Cons length_append length_drop length_rev list.sel(3) nat_neq_iff size_listLength tl_append2)
-          by presburger
-      qed
+       proof(induction "length new < Stack.size (Stack.pop old)")
+         case True
+         then show ?case 
+           by(auto simp: size_pop)
+       next
+         case False
+         then show ?case  
+           apply(auto simp: helper_x)
+           apply (smt (verit, ccfv_SIG) Cons_nth_drop_Suc Stack_Proof.pop Suc_leI Suc_pred append_self_conv2 diff_diff_cancel drop_all_iff leD le_eq_less_or_eq length_drop length_greater_0_conv length_rev less_le_trans list.sel(3) nat_le_linear not_empty_2 ordered_cancel_comm_monoid_diff_class.diff_diff_right size_listLength size_pop take_all tl_append2)
+           by(auto simp: helper_x2)
+       qed
     qed
   next
     case (2 x xs added old remained)
     then show ?case by auto
-  qed
+  qed   
 qed
-  
+
+
 end
